coq, sim: Reduce constant expressions in branches
The RVCore implementation uses expressions in branches, like this:

  Definition getImmediateType : UInternalFunction reg_t empty_ext_fn_t :=
    {{
        fun (inst : bits_t 32) : maybe (enum_t imm_type) =>
          match (inst[|5`d2|:+5]) with
          | #opcode_LOAD[|3`d2|:+5] =>
              {valid (enum_t imm_type)}(enum imm_type {| ImmI |})
          | #opcode_OP_IMM[|3`d2|:+5] =>
              {valid (enum_t imm_type)}(enum imm_type {| ImmI |})
          | #opcode_JALR[|3`d2|:+5] =>
              {valid (enum_t imm_type)}(enum imm_type {| ImmI |})
          | #opcode_AUIPC[|3`d2|:+5] =>
              {valid (enum_t imm_type)}(enum imm_type {| ImmU |})
          | #opcode_LUI[|3`d2|:+5] =>
              {valid (enum_t imm_type)}(enum imm_type {| ImmU |})
          | #opcode_STORE[|3`d2|:+5] =>
              {valid (enum_t imm_type)}(enum imm_type {| ImmS |})
          | #opcode_BRANCH[|3`d2|:+5] =>
              {valid (enum_t imm_type)}(enum imm_type {| ImmB |})
          | #opcode_JAL[|3`d2|:+5] =>
              {valid (enum_t imm_type)}(enum imm_type {| ImmJ |})
          return default: {invalid (enum_t imm_type)}()
          end
    }}.

This desugars to a sequence of ‘if’s whose conditions all have the same form
‘(_mvar == *expr*)’, where *expr* is ‘Binop (IndexedSlice 5) opcode_xxx |3`d2|’.
This commit reduces *expr* (using a small verified interpreter) to be able to
generate a switch on the C++ side.  This changes this:

   if (bool(_mvar == islice<5>(7'0000011_b, 3'010_b))) {
     …
   } else {
     if (bool(_mvar == islice<5>(7'0010011_b, 3'010_b))) {
        …
     …

into this:

   switch (_mvar.v) {
   case 5'00000_bv:
     …
     break;
   case 5'00100_bv:
     …
     break;
   …

ocaml/backends/cpp.ml
@@ -274,17 +274,18 @@ let cpp_preamble =
 let reconstruct_switch action =
   let rec loop v = function
     | Extr.If (_, _,
-              Extr.Binop (_,
-                         (Extr.PrimTyped.Eq _ | Extr.PrimTyped.Bits2 (Extr.PrimTyped.EqBits _)),
-                         Extr.Var (_, v', _, _m),
-                         Extr.Const (_, ((Extr.Bits_t _ | Extr.Enum_t _) as tau), cst)),
-              tbr, fbr) when (match v with
-                              | Some v -> v' = v
-                              | None -> true) ->
-       let default, branches = match loop (Some v') fbr with
-         | Some (_, _, default, branches) -> default, branches
-         | None -> fbr, [] in
-       Some (v', tau, default, (Cuttlebone.Util.value_of_extr_value tau cst, tbr) :: branches)
+               Extr.Binop (_,
+                           (Extr.PrimTyped.Eq _ | Extr.PrimTyped.Bits2 (Extr.PrimTyped.EqBits _)),
+                           Extr.Var (_, v', ((Extr.Bits_t _ | Extr.Enum_t _) as tau), _m),
+                           value),
+               tbr, fbr) when (match v with Some v -> v' = v | None -> true) ->
+       (match Cuttlebone.Util.interp_arithmetic value with
+        | None -> None
+        | Some cst ->
+           let default, branches = match loop (Some v') fbr with
+             | Some (_, _, default, branches) -> default, branches
+             | None -> fbr, [] in
+           Some (v', tau, default, (cst, tbr) :: branches))
     | _ -> None in
   match loop None action with
   | Some (_, _, _, [_]) | None -> None
