coq/ExtractionSetup.v
@@ -28,3 +28,5 @@ Extraction Implicit TypedSyntaxTools.action_mentions_var [R Sigma sig tau].
 Extraction Implicit TypedSyntaxTools.action_mentions_shadowed_var [R Sigma sig tau].
 Extraction Implicit TypedSyntaxTools.existsb_subterm [R Sigma sig tau].
 Extraction Implicit TypedSyntaxTools.is_const_zero [R Sigma sig tau].
+Extraction Implicit TypedSyntaxTools.action_type [R Sigma sig tau].
+Extraction Implicit TypedSyntaxTools.interp_arithmetic [R Sigma sig tau].
